theories/mathcomp_extra.v
@@ -1,0 +1,86 @@
+(* This Source Code Form is subject to the terms of the Mozilla Public
+ * License, v. 2.0. If a copy of the MPL was not distributed with this
+ * file, You can obtain one at https://mozilla.org/MPL/2.0/. *)
+
+(**md**************************************************************************)
+(* # Temporary logical lemmas awaiting inclusion in MathComp                  *)
+(*                                                                            *)
+(* TODO: Move to MCA                                                          *)
+(*                                                                            *)
+(* ```                                                                        *)
+(*        eq4_exists == congruence under four existential quantifiers         *)
+(*              andTP == remove `True` from the left of a conjunction         *)
+(*               ex2C == exchange two existential quantifiers                 *)
+(*               ex3C == exchange the first and third quantifiers             *)
+(*              ex3AC == exchange the second and third quantifiers            *)
+(*            ex_andl == distribute an existential over a right conjunction   *)
+(*            ex_andr == distribute an existential over a left conjunction    *)
+(*             ex_eqr == eliminate a right equality witness                   *)
+(*         ex_eqr_sym == eliminate a symmetric right equality witness         *)
+(*            ex2_eqr == eliminate an equality under two existentials         *)
+(*        ex2_eqr_sym == symmetric version of `ex2_eqr`                       *)
+(* ```                                                                        *)
+(*                                                                            *)
+(******************************************************************************)
+
+From mathcomp Require Import all_boot boolp.
+
+Lemma eq4_exists T S R N
+  (U V : forall (x : T) (y : S x) (z : R x y), N x y z -> Prop) :
+  (forall x y z n, U x y z n = V x y z n) ->
+  (exists x y z n, U x y z n) = (exists x y z n, V x y z n).
+Proof. by move=> UV; apply/eq3_exists => x y z; exact/eq_exists. Qed.
+
+Lemma andTP (P : Prop) : (True /\ P) = P.
+Proof. by apply/propext; split => // -[]. Qed.
+
+Lemma ex2C A B (P : A -> B -> Prop) :
+  (exists a b, P a b) = (exists b a, P a b).
+Proof. by apply/propeqP; split=> -[x [y xy]]; [exists y, x | exists y, x]. Qed.
+
+Lemma ex3C A B C (P : A -> B -> C -> Prop) :
+  (exists a b c, P a b c) = (exists c b a, P a b c).
+Proof.
+apply/propeqP; split=> -[x [y [z xyz]]].
+  by exists z, y, x.
+by exists z, y, x.
+Qed.
+
+Lemma ex3AC A B C (P : A -> B -> C -> Prop) :
+  (exists a b c, P a b c) = (exists a c b, P a b c).
+Proof.
+apply/propeqP; split=> [[a [b [c abc]]] | [a [c [b abc]]]].
+  by exists a, c, b.
+by exists a, b, c.
+Qed.
+
+Lemma ex_andl A (P : A -> Prop) (Q : Prop) :
+  (exists a, P a /\ Q) = ((exists a, P a) /\ Q).
+Proof.
+apply/propeqP; split=> [[a [Pa q]] | [[a Pa] q]].
+  by split=> //; exists a.
+by exists a.
+Qed.
+
+Lemma ex_andr A (P : Prop) (Q : A -> Prop) :
+  (exists a, P /\ Q a) = (P /\ (exists a, Q a)).
+Proof.
+under eq_exists do rewrite andC.
+by rewrite ex_andl andC.
+Qed.
+
+Lemma ex_eqr A (a' : A) (P : A -> Prop) :
+  (exists a, P a /\ a = a') = P a'.
+Proof. by apply/propeqP; split=> [[a [Pa <-//]] | Pa']; exists a'. Qed.
+
+Lemma ex_eqr_sym A (a' : A) (P : A -> Prop) :
+  (exists a, P a /\ a' = a) = P a'.
+Proof. by apply/propeqP; split=> [[a [Pa ->//]] | Pa']; exists a'. Qed.
+
+Lemma ex2_eqr A B (a' : A) (P : A -> B -> Prop) :
+  (exists a b, P a b /\ a = a') = (exists b, P a' b).
+Proof. by rewrite ex2C; apply: eq_exists => b; rewrite ex_eqr. Qed.
+
+Lemma ex2_eqr_sym A B (a' : A) (P : A -> B -> Prop) :
+  (exists a b, P a b /\ a' = a) = (exists b, P a' b).
+Proof. by rewrite ex2C; apply: eq_exists => b; rewrite ex_eqr_sym. Qed.
